

② е) плотность распределения медианы  
выборки

$$f(t) = F'(t)$$

$$Z_{(k)} \sim \sum_{i=k}^n C_n^i F^i(t) (1-F(t))^{n-i} = \Phi(t)$$

$$p(t) = \frac{d}{dt} \Phi(t) = \sum_{i=k}^n C_n^i \left[ i F^{i-1}(t) \cdot f(t) (1-F(t))^{n-i} - (n-i) F^i(t) \cdot (1-F(t))^{n-i-1} \cdot f(t) \right] = f(t) \sum_{i=k}^n C_n^i$$

$$\cdot \left[ i F^{i-1} (1-F)^{n-i} - (n-i) F^i (1-F)^{n-i-1} \right] =$$

$$= f(t) \sum_{i=k}^n \left( \frac{n!}{(i-1)!(n-i)!} F^{i-1} (1-F)^{n-i} - \frac{n!}{i!(n-i-1)!} F^i (1-F)^{n-i-1} \right) =$$

$$= f(t) \left( \frac{n!}{(k-1)!(n-k)!} F^{k-1} (1-F)^{n-k} - \frac{n!}{k!(n-k-1)!} F^k (1-F)^{n-k-1} + \right.$$

$$\left. + \frac{n!}{k!(n-k-1)!} F^k (1-F)^{n-k-1} - \dots - \frac{n!}{n!(n-n-1)!} F^n (1-F)^{n-n-1} \right) =$$

$$= f(t) \cdot \frac{n!}{(k-1)!(n-k)!} \cdot F^{k-1} \cdot (1-F)^{n-k}$$

В нашем случае  $k=13$ ,  $f(t) = e^{-x} \{x \geq 0\}$   
 $n=25$   $F(t) = \int_0^t e^{-t} dt = 1 - e^{-t}$

$$p(t) = \frac{25!}{12!12!} \cdot e^{-t} \cdot (1-e^{-t})^{12} \cdot e^{-12t}$$